theories/simulations/isim/ISimInit.v
@@ -14,7 +14,7 @@ Proof.
   rewrite /state_scopes -!List.map_map alist_upd_keys. eauto.
 Qed.
 
-Lemma isim_refl `{Σ : GRA} r g contextual Ist my_tid fl_src fl_tgt img msk scp
+Lemma isim_refl `{Σ : GRA} r g contextual Ist stid fl_src fl_tgt img msk scp
   ps pt nths st_src st_tgt {R} (it: itree hmodE R)
   (MON: Ist_monotone Ist)
   (EQGET : ∀ nths st_src st_tgt (k: key) (IN: In k.1 scp)
@@ -27,7 +27,7 @@ Lemma isim_refl `{Σ : GRA} r g contextual Ist my_tid fl_src fl_tgt img msk scp
       Ist nths st_src st_tgt -∗ Ist nths (alist_upd k v st_src) (alist_upd k v st_tgt))
   :
   Ist nths st_src st_tgt
-  ⊢ isim contextual fl_src fl_tgt Ist my_tid r g (ist_with_eq Ist) ps pt nths
+  ⊢ isim contextual fl_src fl_tgt Ist stid r g (ist_with_eq Ist) ps pt nths
     (st_src, SB.sandbox img msk scp it)
     (st_tgt, SB.sandbox img msk scp it).
 Proof.
@@ -352,8 +352,8 @@ Section Proph.
   Variable contextual: contextuality.
 
   Lemma isim_fsem_proph_to_normal fsp bd_s bd_t msk sp scp fls flt
-    (SIM: ∀ arg my_tid nths st (TID: my_tid < nths),
-        ⊢ isim contextual fls flt IstEq my_tid ibot ibot (ist_with_eq IstEq) true true nths
+    (SIM: ∀ arg stid nths st (TID: stid < nths),
+        ⊢ isim contextual fls flt IstEq stid ibot ibot (ist_with_eq IstEq) true true nths
           (st, SB.sandbox true  msk scp (SModTr.trans sp      (bd_s arg)))
           (st, SB.sandbox false msk scp (SModTr.trans sp_none (bd_t arg))))
     :
